# Comparison between for loops and pattern matching

A common problem many beginners in functional programming have is that, at first glance, we lost the ability to do for loops. This blog post will showcase a number of for loops and compare them with their functional counterpart.

## Iterating through a collection

I'm sure most of you have met something like the following form before:

```python
for x in xs:
    update_state(state, x)
return state;
```

It's often built on top of iterators, let's "desugar" it step by step. I will use Java here:

```java
for (Foo x: collectionOfFoo)
    do_something_with(state, x);
return state;

// into
val iter = collectionOfFoo.iterator();
while (iter.hasNext()) {
    val x = iter.peek();
    do_something_with(state, x);
    iter.next();
}
return state;
```

Notice in each iteration, we are updating the state, and we are given an iterator that can either be empty or has a head. We then "reduce" the iterator by striping its head until it's empty. We will do the exact same thing in Haskell.

```haskell
f [] state     = state                              -- "return"
f (x:xs) state = f xs (do_something_with state x)   -- execute the body and go to next iteration
-- ^  ^
-- | iter = "iter.stripHead"
-- iter.next   
```

Note how the `do_something_with` is the same, but the "goto" part implied by the while loop is done via recursion.

## Do something x times

Let's look at "do something x times" kind of loop, this is probably missed the most, but as we are about to see, the imperative version is very verbose and lacks sugar like in the iteration case above.

```c
int fib(int n) {
    int x = 1;
    int y = 1;
    for (int i = 0; i < n - 1; i++) {
        int tmp = y;
        y += x;
        x = tmp;
    }
    return y;
}
```

We shall see that we can have a tail-recursive version in Haskell that's just as fast, but much shorter.

```haskell
fib n = fib' 0 1 n
    where
        fib' _ y 0 = y
        fib' x y n' = fib' y (x + y) (n' - 1)
```

## Indexed for loop

```java
for (int i = 0; i < xs.length; i++)
    do_something_with(i, xs[i], state)
```

```haskell
f xs state = f' (zip xs [1..xs.length]) state
    where
        f' [] state     = state
        f' ((x, i):xs) state = f xs (do_something_with state x i)
```

Notice how the imperative version needs a bit more code when it lost the iterator sugar, but the functional version stayed mostly the same. (And of course a fold would be much more convenient here)
